theories/CombinatoryLogic/Plotkin.v
@@ -23,7 +23,7 @@ Fixpoint cbv_cbn (t : term) : term :=
 Definition Psi (t : term) :=
   match t with
   | var n => var n
-  | app s t => app s t
+  | app s t => lam (app (var 0) (cbv_cbn (app s t)))
   | lam s => lam (cbv_cbn s)
   end.
 
@@ -46,6 +46,383 @@ Proof.
     congr lam. congr app. congr lam.
     admit.
 Admitted.
+
+
+Lemma cbv_cbn_ren xi s : cbv_cbn (ren xi s) = ren xi (cbv_cbn s).
+Proof.
+  elim: s xi.
+  - done.
+  - move=> ? IH1 ? IH2 xi /=. by rewrite IH1 IH2 !simpl_term.
+  - move=> ? IH xi /=. rewrite IH !simpl_term.
+    congr lam. congr app. congr lam.
+    apply: ext_ren_term. by case.
+Qed.
+
+(* TODO proof could be simplified ? *)
+Lemma cbv_cbn_subst sigma s : 
+  (forall n, match sigma n with | app _ _ => False | _ => True end) ->
+  cbv_cbn (subst sigma s) = subst (funcomp Psi sigma) (cbv_cbn s).
+Proof.
+  elim: s sigma.
+  - move=> n sigma Hsigma /=.
+    have := Hsigma n. by case: (sigma n).
+  - move=> s IH1 t IH2 sigma Hsigma /=.
+    rewrite (IH1 _ Hsigma) (IH2 _ Hsigma) /=.
+    rewrite !simpl_term /=.
+    congr lam. congr app. congr lam. congr app.
+    apply: ext_subst_term => ? /=. by rewrite !simpl_term.
+  - move=> s IH sigma Hsigma /=.
+    rewrite IH.
+    { move=> [|n] /=; first done.
+      have := Hsigma n. by case: (sigma n). }
+    rewrite !simpl_term.
+    congr lam. congr app. congr lam.
+    apply: ext_subst_term => - [|n] /=; first done.
+    have := Hsigma n. case: (sigma n); [done|done|].
+    move=> s' /= _. rewrite !cbv_cbn_ren.
+    congr lam. rewrite !simpl_term. apply: ext_ren_term.
+    by case.
+Qed.
+
+Fixpoint colon' s t :=
+  match s with
+  | var _ => app t (Psi s)
+  | lam _ => app t (Psi s)
+  | app s1 s2 =>
+      colon' s1 (lam (app (ren S (cbv_cbn s2)) (lam (app (app (var 1) (var 0)) (ren S (ren S t))))))
+  end.
+
+Import Relation_Operators (t1n_trans).
+
+Lemma stepsf_to_colon' s u : exists n, stepsf (S n) (app (cbv_cbn s) u) = Some (colon' s u).
+Proof.
+  elim: s u.
+  - move=> n u /=. by exists 0.
+  - move=> s IH1 t IH2 u /=.
+    have [n Hn] := IH1 (lam (app (ren S (cbv_cbn t)) (lam (app (app (var 1) (var 0)) (ren S (ren S u)))))).
+    exists (S n). rewrite -Hn.
+    rewrite (stepsf_plus 1 (S n)) /=.
+    by rewrite !simpl_term /= !ren_as_subst_term.
+  - move=> ???. exists 0. move=> /=.
+    rewrite /stepsf /= !simpl_term /=. congr Some. congr app. congr lam.
+    rewrite -[RHS]subst_var_term. apply: ext_subst_term. by case.
+Qed.
+
+
+Lemma colon'_top_level_redex s t u :
+  exists n, stepsf (S n) (colon' (app (lam s) (lam t)) u) = 
+    Some (colon' (subst (scons (lam t) var) s) u).
+Proof.
+  have [n <-] := stepsf_to_colon' ((subst (scons (lam t) var) s)) u.
+  exists (4+n). rewrite (stepsf_plus 4 (S n)).
+  rewrite cbv_cbn_subst. { by case. }
+  rewrite /stepsf /=.
+  congr obind. congr Nat.iter. congr Some.
+  rewrite !simpl_term /=. congr app.
+  apply: ext_subst_term.
+  case; last done.
+  congr lam.
+  rewrite -[RHS]subst_var_term.
+  apply: ext_subst_term. by case.
+Qed.
+
+
+Lemma redex_colon' s t u : 
+  exists n, stepsf (S n) (app (app (lam (cbv_cbn s)) (lam (cbv_cbn t))) u) =
+    Some (colon' (subst (scons (lam t) var) s) u).
+Proof.
+  have [n Hn] := stepsf_to_colon' (subst (scons (lam t) var) s) u.
+  exists (S n).
+  rewrite (stepsf_plus 1 (S n)) -Hn /=.
+  rewrite cbv_cbn_subst /=. { by case. }
+  congr stepsf. congr app.
+  apply: ext_subst_term. by case.
+Qed.
+
+Lemma closed_eval {s t} : L.eval s t -> closed s -> closed t.
+Proof. by move=> /eval_iff [/closed_star]. Qed.
+
+Arguments colon' : simpl never.
+
+Lemma bound_ren {k k' xi t} : bound k t -> (forall n, n < k -> xi n < k') -> bound k' (ren xi t).
+Proof.
+  elim: t k k' xi.
+  - move=> > /boundE ? H /=. apply: dclvar. by apply: H.
+  - move=> ? IH1 ? IH2 > /boundE + ? /=.
+    move=> [/IH1 {}IH1 /IH2 {}IH2]. apply: dclApp; [by apply: IH1|by apply: IH2].
+  - move=> ? IH > /boundE /IH {}IH H /=.
+    apply: dcllam. apply: IH.
+    move=> [|n] /=; [|have := H n]; lia.
+Qed.
+
+Lemma bound_subst {k k' sigma t} : bound k t -> (forall n, n < k -> bound k' (sigma n)) -> bound k' (subst sigma t).
+Proof.
+  elim: t k k' sigma.
+  - move=> > /boundE ? H /=. by apply: H.
+  - move=> ? IH1 ? IH2 > /boundE + ? /=.
+    move=> [/IH1 {}IH1 /IH2 {}IH2]. apply: dclApp; [by apply: IH1|by apply: IH2].
+  - move=> ? IH > /boundE /IH {}IH H /=.
+    apply: dcllam. apply: IH.
+    move=> [|n] /=.
+    + move=> _. apply: dclvar. lia.
+    + move=> ?. apply: bound_ren.
+      * apply: H. lia.
+      * lia.
+Qed.
+
+Lemma bound_cbv_cbn k t : bound k t -> bound k (cbv_cbn t).
+Proof.
+  elim: t k.
+  - move=> n k /boundE H. rewrite /cbv_cbn. apply: dcllam.
+    apply: dclApp; apply: dclvar; lia.
+  - move=> ? IH1 ? IH2 k /boundE [/IH1 {}IH1 /IH2 {}IH2] /=.
+    apply: dcllam. apply: dclApp.
+    + apply: (bound_ren IH1). lia.
+    + apply: dcllam. apply: dclApp.
+      * rewrite !simpl_term /=. apply: (bound_ren IH2). lia.
+      * apply: dcllam. apply: dclApp; [apply: dclApp|]; apply: dclvar; lia.
+  - move=> ? IH k /boundE /IH {}IH /=.
+    apply: dcllam. apply: dclApp; [apply: dclvar; lia|].
+    apply: dcllam. apply: (bound_ren IH).
+    move=> [|n] /=; lia.
+Qed.
+
+(* cbv simulation lemma for closed terms *)
+Lemma main_forward s t : L.eval s t -> closed s ->
+  forall x, exists n, stepsf n (colon' s x) = Some (colon' t x).
+Proof.
+  elim. { move=> ???. by exists 0. }
+  move=> {}s u {}t t' v Hsu IH1 Htt' IH2 Hv IH3 /closed_app [Hs Ht].
+  move=> /(_ Hs) in IH1. move=> /(_ Ht) in IH2.
+  have Ht' : closed t' by (apply: closed_eval; eassumption).
+  have Hu : bound 1 u.
+  { by have /closed_dcl /boundE := closed_eval Hsu Hs. } 
+  have /IH3 {}IH3 : closed (L.subst u 0 t').
+  { apply /closed_dcl. apply: closed_subst; [done|by apply /closed_dcl]. }
+  move=> x.
+  move: IH3.
+  have -> : L.subst u 0 t' = subst (scons t' var) u.
+  { rewrite L_subst_subst; first done.
+    apply: (bound_ext_subst_term Hu).
+    move=> [|n]; [done|lia]. }
+  move: Htt' {Hv} IH2 Ht' => /eval_iff [_] [] t'' -> IH2 Ht'' IH3.
+  pose x1 := lam (app (ren S (cbv_cbn t)) (lam (app (app (var 1) (var 0)) (ren S (ren S x))))).
+  pose x2 := lam (app (app (lam (cbv_cbn u)) (var 0)) (ren S x)).
+  have -> : colon' (app s t) x = colon' s x1 by done.
+  have [n1 Hn1] := IH1 x1.
+  have H'n1 : stepsf 1 (colon' (lam u) x1) = Some (app (cbv_cbn t) x2).
+  { rewrite /stepsf /= /x2. congr Some. rewrite !simpl_term !ren_as_subst_term /=.
+    congr app. congr lam. congr app. congr app. congr lam.
+    move: Hu => /bound_cbv_cbn /bound_ext_subst_term.
+    rewrite -[RHS]subst_var_term. apply.
+    move=> [|?] /=; [done|lia]. }
+  have [n2 Hn2] := stepsf_to_colon' t x2.
+  have [n3 Hn3] := IH2 x2.
+  have H'n3 : stepsf 1 (colon' (lam t'') x2) = Some (app (app (lam (cbv_cbn u)) (lam (cbv_cbn t''))) x).
+  { rewrite /stepsf /= /x2. congr Some. rewrite !simpl_term /=.
+    congr app. congr app. congr lam.
+    move: Hu => /bound_cbv_cbn /bound_ext_subst_term.
+    rewrite -[RHS]subst_var_term. apply.
+    move=> [|?] /=; [done|lia]. }
+  have [n4 Hn4] := redex_colon' u t'' x.
+  have [n5 Hn5] := IH3 x.
+  exists (n1 + (1 + (S n2 + (n3 + (1 + (S n4 + n5)))))).
+  rewrite stepsf_plus Hn1 /=.
+  rewrite (stepsf_plus 1 (S n2 + (n3 + (1 + (S n4 + n5))))) H'n1 /=.
+  rewrite (stepsf_plus (S n2) (n3 + (1 + (S n4 + n5)))) Hn2 /=.
+  rewrite (stepsf_plus n3 (1 + (S n4 + n5))) Hn3 /=.
+  rewrite (stepsf_plus 1 (S n4 + n5)) H'n3 /=.
+  by rewrite (stepsf_plus (S n4) n5) Hn4 /=.
+Qed.
+
+Print Assumptions main_forward.
+
+(* BACKWARD DIRECTION using leftmost outermost L step *)
+
+Definition is_app (t : term) :=
+  if t is app _ _ then true else false.
+
+(* left-most outer-most cbv step *)
+Fixpoint cbv_stepf (s : term) : option term :=
+  match s with
+  | app s t =>
+      match cbv_stepf s with
+      | Some s' => Some (app s' t)
+      | None =>
+          if is_app s then None else
+            match cbv_stepf t with
+            | Some t' => Some (app s t')
+            | None =>
+                match s, t with
+                | lam s', lam t' => Some (subst (scons (lam t') var) s')
+                | _, _ => None
+                end
+            end
+      end
+  | _ => None
+  end.
+
+Definition cbv_stepsf k s := Nat.iter k (obind cbv_stepf) (Some s).
+
+Arguments cbv_stepsf : simpl never.
+Arguments cbv_stepf : simpl never.
+
+Lemma cbv_stepsf_plus n m s : cbv_stepsf (n + m) s = (obind (cbv_stepsf m)) (cbv_stepsf n s).
+Proof.
+  rewrite /cbv_stepsf iter_plus. case: (Nat.iter n _ _); [done|by rewrite oiter_None].
+Qed.
+
+Lemma cbv_stepsf_appL {k s s' t} :
+  cbv_stepsf k s = Some s' ->
+  cbv_stepsf k (app s t) = Some (app s' t).
+Proof.
+  elim: k s s' t. { by move=> > [<-]. }
+  move=> k IH s s' t.
+  rewrite !(cbv_stepsf_plus 1 k).
+  rewrite /(cbv_stepsf 1) /=.
+  case E: (cbv_stepf s) => [s''|]; last done.
+  move=> /= /IH {}IH.
+  rewrite /cbv_stepf -/cbv_stepf E. by apply: IH.
+Qed.
+
+Lemma cbv_stepsf_appR {k s t t'} :
+  cbv_stepsf k t = Some t' ->
+  cbv_stepsf k (app (lam s) t) = Some (app (lam s) t').
+Proof.
+  elim: k s t t'. { by move=> > [<-]. }
+  move=> k IH s t t'.
+  rewrite !(cbv_stepsf_plus 1 k).
+  rewrite /(cbv_stepsf 1) /=.
+  case E: (cbv_stepf t) => [t''|]; last done.
+  move=> /= /IH {}IH.
+  rewrite /cbv_stepf -/cbv_stepf E. by apply: IH.
+Qed.
+
+(* this can be used to simplify forward direction proof *)
+Lemma eval_cbv_stepsf s t : L.eval s t -> closed s -> exists k, cbv_stepsf k s = Some t.
+Proof.
+  elim; clear s t. { move=> *. by exists 0. }
+  move=> s u t t' v Hsu IH1 Htt' IH2 Hv IH3 /closed_app [Hs Ht].
+  move: (Hs) => /IH1 => - [k1 {}IH1].
+  move: (Ht) => /IH2 => - [k2 {}IH2].
+  have Ht' : closed t' by (apply: closed_eval; eassumption).
+  have Hu : bound 1 u.
+  { by have /closed_dcl /boundE := closed_eval Hsu Hs. } 
+  have /IH3 [k3 {}IH3] : closed (L.subst u 0 t').
+  { apply /closed_dcl. apply: closed_subst; [done|by apply /closed_dcl]. }
+  move: IH3.
+  have -> : L.subst u 0 t' = subst (scons t' var) u.
+  { rewrite L_subst_subst; first done.
+    apply: (bound_ext_subst_term Hu).
+    move=> [|n]; [done|lia]. }
+  move=> <-. exists (k1 + (k2 + S k3)).
+  rewrite cbv_stepsf_plus (cbv_stepsf_appL IH1) /=.
+  rewrite cbv_stepsf_plus (cbv_stepsf_appR IH2) /=.
+  rewrite (cbv_stepsf_plus 1 k3) /=.
+  by move: Htt' => /eval_iff [_] [? ->].
+Qed.
+
+Lemma cbv_stepf_closed {s s'} : cbv_stepf s = Some s' -> closed s -> closed s'.
+Proof.
+  elim: s s'; [done| |done].
+  move=> s IH1 t IH2 s'. rewrite /cbv_stepf -/cbv_stepf.
+  case Es: (cbv_stepf s) => [s''|].
+  { move=> [<-] /closed_app [? ?].
+    apply: app_closed; last done.
+    by apply: IH1. }
+  case: (is_app s); first done.
+  case Et: (cbv_stepf t) => [t''|].
+  { move=> [<-] /closed_app [? ?].
+    apply: app_closed; first done.
+    by apply: IH2. }
+  case: (s); [done|done|] => ?.
+  case: (t); [done|done|] => ?.
+  move=> [<-] /closed_app [/closed_dcl /boundE ?] /closed_dcl ?.
+  apply /closed_dcl. apply: bound_subst; first by eassumption.
+  move=> [|n]; [done|lia].
+Qed.
+
+Lemma cbv_stepf_step s s' : cbv_stepf s = Some s' -> closed s -> L_facts.step s s'.
+Proof.
+  elim: s s'; [done| |done].
+  move=> s IH1 t IH2 s'. rewrite /cbv_stepf -/cbv_stepf.
+  case Es: (cbv_stepf s) => [s''|].
+  { move=> [<-] /closed_app [? ?].
+    apply: stepAppL. by apply: IH1. }
+  case: (is_app s); first done.
+  case Et: (cbv_stepf t) => [t''|].
+  { move=> [<-] /closed_app [? ?].
+    apply: stepAppR. by apply: IH2. }
+  case: (s); [done|done|] => s'''.
+  case: (t); [done|done|] => t'''.
+  move=> [<-] /closed_app [/closed_dcl /boundE ?] /closed_dcl ?.
+  have := L_facts.stepApp s''' t'''. congr L_facts.step.
+  rewrite L_subst_subst. { by apply /closed_dcl. }
+  apply: bound_ext_subst_term; first by eassumption.
+  move=> [|n]; [done|lia].
+Qed.
+
+Lemma cbv_stepsf_eval k s t : cbv_stepsf k s = Some (lam t) -> closed s -> L.eval s (lam t).
+Proof.
+  move=> Hk Hs. apply /eval_iff. split; last done.
+  elim: k s t Hk Hs.
+  { move=> > [->] ?. by apply: starR. }
+  move=> k IH s t.
+  rewrite (cbv_stepsf_plus 1 k) /(cbv_stepsf 1) /=.
+  case E: (cbv_stepf s) => [s'|]; last done.
+  move=> + Hs. move: (Hs) => /(cbv_stepf_closed E) /IH /[apply] ?.
+  apply: starC; last by eassumption.
+  by apply: cbv_stepf_step.
+Qed.
+
+Lemma simulate_cbv_stepf s t : cbv_stepf s = Some t ->
+  forall x, exists k, stepsf (S k) (colon' s x) = Some (colon' t x).
+Proof.
+  elim: s t; [done| |done].
+  move=> s1 IH1 s2 IH2 t. rewrite /cbv_stepf -/cbv_stepf.
+  case Es1: (cbv_stepf s1) => [s1'|].
+  { move=> [<-] x.
+    move: Es1 => /IH1 {}IH1.
+    by apply: IH1. }
+  case Hs1: (is_app s1); first done.
+  case Es2: (cbv_stepf s2) => [s2'|].
+  { move=> [<-] x.
+    have H's1 : forall t, colon' (app s1 t) x = app (lam (app (ren S (cbv_cbn t)) (lam (app (app (var 1) (var 0)) (ren S (ren S x)))))) (Psi s1).
+    { by case: (s1) Hs1. }
+    rewrite !H's1. move: Es2 => /IH2 {}IH2.
+    (* does not work immediately, needs more complicated colon as by plotkin?
+    or just different stepf? *)
+    
+    
+    }
+
+  admit. (* doesnt work because of nested left apps that have no redex *) }
+  case: (s1); [done|done|] => s1''.
+  case: (s2); [done|done|] => s2''.
+  move=> [<-] x. have [k Hk] := colon'_top_level_redex s1'' s2'' x.
+  exists k. apply: Hk.
+Admitted.
+
+(**
+(* OBSOLETE  *)
+
+Lemma colon'_top_level_redex s t u : clos_trans step (colon' (app (lam s) (lam t)) u) (colon' (subst (scons (lam t) var) s) u).
+Proof.
+  move=> /=.
+  apply /clos_trans_t1n_iff. apply: t1n_trans. { by apply: stepLam. }
+  rewrite /=. apply: t1n_trans. { by apply: stepLam. }
+  rewrite /=. apply: t1n_trans. { by apply: stepLam. }
+  rewrite /=. apply: t1n_trans. { apply: stepApp. by apply: stepLam. }
+  apply /clos_trans_t1n_iff.
+  have := asd0 ((subst (scons (lam t) var) s)) u.
+  congr clos_trans. rewrite cbv_cbn_subst. { by case. }
+  rewrite !simpl_term. congr app; [|by rewrite -[LHS]subst_var_term].
+  apply: ext_subst_term.
+  case; last done.
+  congr lam.
+  rewrite -[LHS]subst_var_term.
+  apply: ext_subst_term. by case.
+Qed.
 
 (*
 Lemma lemma_6_1 M N :
@@ -172,11 +549,7 @@ Proof.
 Admitted.
 *)
 
-Lemma bound_cbv_cbn k t : bound k t -> bound k (cbv_cbn t).
-Proof.
-  elim: t.
-  - move=> n H. rewrite /cbv_cbn.
-Admitted.
+
 
 Lemma closed_cbv_cbn t : closed t -> closed (cbv_cbn t).
 Proof. Admitted.
@@ -251,6 +624,9 @@ Proof.
   by case: n.
 Qed.
 
+
+
+
 Lemma main_backward s :
   closed s -> clos_refl_trans step (colon s u) (colon (lam t) u) -> 
   
@@ -269,3 +645,4 @@ Proof.
   Print or.
 
 Check Seval.stepf.
+*)
